\documentclass{article}
\usepackage{ifthen}
\usepackage{epsfig}
\usepackage[utf8]{inputenc}
\usepackage{newunicodechar}
  \newunicodechar{⁻}{${}^{-}$}% Superscript minus
  \newunicodechar{²}{${}^{2}$}% Superscript two
  \newunicodechar{³}{${}^{3}$}% Superscript three

\pagestyle{empty}
\begin{document}
\[ e = \max \left( \frac{|x(k) - y(k)| }{ |x(k)|} \right), \quad \quad |x(k)| > 0, \]
\pagebreak

\[ e = \max(|x(k) - y(k)| ), ~\qquad \quad~|x(k)| = 0, \]
\pagebreak

$ e$
\pagebreak

$ C_ord(x)$
\pagebreak

\[ C_ord(x) = 2 x C_{ord-1}(x) - C_{ord-2}(x), \]
\pagebreak

$ C_0(x) = 1 $
\pagebreak

$ C_1(x) = x$
\pagebreak

$ U_{ord}(x)$
\pagebreak

\[ U_{ord}(x) = 2 x U_{ord-1}(x) - U_{ord-2}(x), \]
\pagebreak

$ U_0(x) = 1 $
\pagebreak

$ U_1(x) = 2x$
\pagebreak

$ x = a + j b $
\pagebreak

\[ |x|^2 = x x^* = a^2 + b^2. \]
\pagebreak

\[ \textrm{Arccos}(x) = \frac{\pi}{2} - \textrm{Arcsin}(x) = \frac{\pi}{2} -j \textrm{Ln}\left( j x + \sqrt{1 - x^2} \right) \]
\pagebreak

\[ \textrm{Arcsin}(x) = j \textrm{Ln}\left( j x + \sqrt{1 - x^2} \right) \]
\pagebreak

\[ \textrm{cos}(x) = \frac{\exp(jx) + \exp(-jx)}{2} \]
\pagebreak

\[ \textrm{Ln}(x) = j \varphi + \ln(|x|), \]
\pagebreak

$\varphi$
\pagebreak

\[ \textrm{sin}(x) = \frac{\exp(jx) - \exp(-jx)}{2j} \]
\pagebreak

\[ y(k) = \sqrt{x(k)}, \qquad k = 0 \ldots n-1. \]
\pagebreak

$ c = a * b$
\pagebreak

$a$
\pagebreak

$b$
\pagebreak

$n = n_0 \times n_1 \times n_2 \times n_3 \times \ldots \times n_p \times m$
\pagebreak

$n_i = 2,3,5,7$
\pagebreak

$m $
\pagebreak

\[ H(z) = \frac{\sum_{n = 0}^{N} b_n z^{-n}} {1+{\frac{1}{a_0}}\sum_{m = 1}^{M} a_m z^{-m}}, \]
\pagebreak

$a_0$
\pagebreak

$N=M=$
\pagebreak

$s(t) = \sin(2\pi \cdot 0.05 t) + n(t)$
\pagebreak

$n(t)$
\pagebreak

$ n $
\pagebreak

$ x(m) $
\pagebreak

$ m = 0 \ldots n-1 $
\pagebreak

\[ Y(k) = \sum_{m = 0}^{n-1} x(m) \exp \left( -j \frac{2\pi}{n} m k \right), \]
\pagebreak

$ k = 0 \ldots n-1 $
\pagebreak

$x(m)$
\pagebreak

$n$
\pagebreak

$Y(k)$
\pagebreak

$ n^2 $
\pagebreak

\[ y(k) = \sum_{m = 0}^{n-1} x(m) \exp \left( j \frac{2\pi}{n} m k \right), \]
\pagebreak

$y(k)$
\pagebreak

$ u = \textrm{cd}^{-1}(w, k)$
\pagebreak

$ w $
\pagebreak

$ k $
\pagebreak

$ u = \textrm{sn}^{-1}(w, k)$
\pagebreak

$ y = \textrm{cd}(u K(k), k)$
\pagebreak

$ u $
\pagebreak

$ k_i $
\pagebreak

$ K(k) $
\pagebreak

\[ K(k) = \frac{\pi}{2} \prod_{i = 1}^{\infty}(1+k_i), \]
\pagebreak

$ k_0 = k$
\pagebreak

\[ k_i = \left( \frac{k_{i-1}} { 1+\sqrt{1-k_{i-1}^2} } \right)^2 \]
\pagebreak

$ k<1 $
\pagebreak

$ y = \textrm{sn}(u K(k), k)$
\pagebreak

\[ Y(k) = \frac{1}{N} \sum_{m = 0}^{n-1} x(m) \exp \left( j \frac{2\pi}{n} m k \right), \]
\pagebreak

$ n = 725760 $
\pagebreak

$725760 = 2 \cdot 3 \cdot 4 \cdot 5 \cdot 6 \cdot 7 \cdot 9 \cdot 16 $
\pagebreak

$ n = 172804 = 43201 \cdot 4 $
\pagebreak

$ n = 13 \cdot 17 \cdot 23 \cdot 13 = 66079 $
\pagebreak

$\sqrt{2^{31}} = 46340.95$
\pagebreak

$x_0$
\pagebreak

$x_1$
\pagebreak

$x(k) = x_0 + k \cdot dx$
\pagebreak

$dx = \frac{x_1 - x_0}{n-1}$
\pagebreak

$k = 0 \ldots n-1.$
\pagebreak

$dx = \frac{x_1 - x_0}{n}$
\pagebreak

$10^{x_0}$
\pagebreak

$10^{x_1}$
\pagebreak

$x(k) = 10^{x_0} \cdot dx^k$
\pagebreak

$dx = \sqrt[n-1]{10^{x_1 - x_0}}$
\pagebreak

$dx = \sqrt[n]{10^{x_1 - x_0}}$
\pagebreak

$ H(j \omega) $
\pagebreak

$ H(j \omega)$
\pagebreak

$ H(s) $
\pagebreak

\[ H(s) = \frac {\sum_{k = 0}^{N} b_k s^k} {\sum_{m = 0}^{N} a_m s^m}, \]
\pagebreak

$ N $
\pagebreak

$ s = j \omega $
\pagebreak

$ \omega $
\pagebreak

$H(s)$
\pagebreak

$H(z)$
\pagebreak

$ H \left(\mathrm{e}^{j\omega} \right) $
\pagebreak

$ 2\pi $
\pagebreak

$ \pi $
\pagebreak

$ -\pi $
\pagebreak

$ H \left(e^{j \omega} \right)$
\pagebreak

\[ H(z) = \frac {\sum_{k = 0}^{N} b_k z^{-k}} {\sum_{m = 0}^{N} a_m z^{-m}}, \]
\pagebreak

$N$
\pagebreak

$z = e^{j \omega} $
\pagebreak

$\omega$
\pagebreak

$ 2 \pi-$
\pagebreak

$2 \pi$
\pagebreak

$-\pi$
\pagebreak

$ \pi$
\pagebreak

$ H \left(e^{j \omega} \right) = H^* \left(e^{-j \omega} \right)$
\pagebreak

$\pi$
\pagebreak

$ -R_p $
\pagebreak

$ H(s)$
\pagebreak

$-R_p$
\pagebreak

$ R_p $
\pagebreak

$-R_s$
\pagebreak

$H(j\cdot 1) = -R_s$
\pagebreak

\[ H(s) = \frac{\sum_{n = 0}^{N_z} b_n \cdot s^n}{\sum_{m = 0}^{N_p} a_m \cdot s^m} = \frac{\prod_{n = 0}^{N_z}(s-z_n)}{\prod_{m = 0}^{N_p} (s-p_m)} \]
\pagebreak

$ F(s) $
\pagebreak

$F(s)$
\pagebreak

$Y(s) = (H \circ F)(s) = H(F(s))$
\pagebreak

\[ H(s) = \frac{\sum\limits_{m = 0}^{n} b_m s^m}{\sum\limits_{k = 0}^{n} a_k s^k}, \quad F(s) = \frac{\sum\limits_{m = 0}^{p} d_m s^m}{\sum\limits_{k = 0}^{p} c_k s^k}, \quad Y(s) = \frac{\sum\limits_{m = 0}^{n p} \beta_m s^m}{\sum\limits_{k = 0}^{n p} \alpha_k s^k} \]
\pagebreak

$Y(s) = (H \circ F)(s)$
\pagebreak

\[ s \leftarrow \frac{1 - z^{-1}}{1 - z^{-1}}. \]
\pagebreak

$\Omega$
\pagebreak

\[ \Omega = \tan(\omega / 2). \]
\pagebreak

\[ s(t) = \sum\limits_{n = 0}^{n_{\omega}-1} S(\omega_n) \exp(j\omega_n t) \]
\pagebreak

$\omega_n$
\pagebreak

$S(\omega_n)$
\pagebreak

$ I_0(x)$
\pagebreak

$ x $
\pagebreak

$[0 \ 3]$
\pagebreak

$ \textrm{sinc}(x,a) = \frac{\sin(ax)}{ax}$
\pagebreak

\[ \textrm{Si}(x) = \int_{0}^{x} \frac{\sin(x)}{x} \, dx\]
\pagebreak

$[-6\pi \ 6\pi]$
\pagebreak

$a_{ij}$
\pagebreak

$P_N(x)$
\pagebreak

$N-$
\pagebreak

\[ P_N(x) = a_0 + a_1 \cdot x + a_2 \cdot x^2 + a_3 \cdot x^3 + ... a_N \cdot x^N. \]
\pagebreak

\[ P_N(x) = a_0 + x \cdot (a_1 + x \cdot (a_2 + \cdot ( \ldots x \cdot (a_{N-1} + x\cdot a_N) \ldots ))) \]
\pagebreak

$10^{56}$
\pagebreak

\end{document}
